Made wp a first-class nola object

nola/examples/awp.v
@@ -15,17 +15,83 @@ Section awp.
 
   Local Notation "'aProp'" := (aProp CON JUDG Σ).
 
-
-  About wp.
-
-  Definition awp {b} s E e (Φ : _ -> aProp b) := wpw (inv_wsat ⟦⟧ᶜ) s E e%E (λ v, aProp_to_iProp_deriv der (Φ v)).
-  Definition atwp {b} s E e (Φ : _ -> aProp b) := twpw (inv_wsat ⟦⟧ᶜ) s E e%E (λ v, aProp_to_iProp_deriv der (Φ v)).
+  Definition awp b s E e (Φ : _ -> aProp b) := wpw (inv_wsat ⟦⟧ᶜ) s E e%E (λ v, aProp_to_iProp_deriv der (Φ v)).
+  Definition atwp b s E e (Φ : _ -> aProp b) := twpw (inv_wsat ⟦⟧ᶜ) s E e%E (λ v, aProp_to_iProp_deriv der (Φ v)).
 
 
   Lemma atwp_awp {b} s E e (Φ : _ -> aProp b) :
-    atwp s E e Φ ⊢ awp s E e Φ.
+    atwp b s E e Φ ⊢ awp b s E e Φ.
   Proof.
     apply twpw_wpw.
   Qed.
 
 End awp.
+
+Section custom_wp.
+
+  Context `{!Csem CON JUDG Σ, Jsem JUDG (iProp Σ)}.
+  Context `{!lrustGS_gen hlc Σ}.
+  Context `{!inv'GS (cifOF CON) Σ}.
+
+  (** ** Custom constructors *)
+
+  (** [customCT]: Constructor *)
+  Variant customCT_id := .
+  Variant customCT_sel :=
+  | (** WP token *) cifs_wp (b : bool) (s : stuckness) (E : coPset) (e : language.expr lrust_lang) (Φ : language.val lrust_lang → aProp CON JUDG Σ b)
+  | (** Total WP token *) cifs_twp (b : bool) (s : stuckness) (E : coPset) (e : language.expr lrust_lang) (Φ : language.val lrust_lang → aProp CON JUDG Σ b).
+  Arguments cifs_wp {_}.
+  Arguments cifs_twp {_}.
+
+  Definition customCT := Cifcon customCT_id (customCT_sel)
+  (λ _, Empty_set) (λ _, Empty_set) (λ _, unitO) _.
+  (** [customC]: [customCT] registered *)
+  (*
+      [inC : cifcon → cifcon → Type]
+      To be understood as the inclusion of one custom constructor
+      structure for [cif] into another.
+  *)
+  Notation customC := (inC customCT).
+  Section customC.
+    Context `{!customC CON}.
+    (** [cif_wp]: WP token *)
+    Definition cif_wp {b} s E e Φ : cif CON Σ :=
+      cif_in customCT ( @cifs_wp b s E e Φ) nullary nullary ().
+    (** [cif_twp]: TWP token *)
+    Definition cif_twp {b} s E e Φ : cif CON Σ :=
+      cif_in customCT ( @cifs_twp b s E e Φ) nullary nullary ().
+
+    (** Semantics of [customCT] *)
+    Definition customCT_sem (s : customCT_sel) : iProp Σ :=
+      match s with
+      | @cifs_wp b s E e Φ => awp b s E e Φ
+      | @cifs_twp b s E e Φ => atwp b s E e Φ
+      end.
+    #[export] Program Instance customCT_ecsem
+      : Ecsem customCT CON JUDG Σ :=
+      ECSEM (λ _ _ s _ _ _, customCT_sem s) _.
+    Next Obligation (* Proof of non-expansiveness *). done. Qed.
+  End customC.
+  (** [customC] semantics registered *)
+  (*
+      [inCS : ∀ (CON' CON : cifcon) (JUDG : ofe) Σ,
+        inC CON' CON →
+        Ecsem CON' CON JUDG Σ →
+        Csem CON JUDG Σ → Prop]
+      To be understood as the inclusion of the semantics.
+  *)
+  Notation customCS := (inCS customCT).
+
+  Section customC.
+    Context `{!customC CON, !customCS CON JUDG Σ}.
+
+    (** Reify token *)
+    #[export] Program Instance wp_as_cif {b} s E e Φ :
+        AsCif CON (λ _, awp b s E e Φ)%I := AS_CIF (cif_wp s E e Φ) _.
+    Next Obligation. move=>/= >. by rewrite sem_cif_in. Qed.
+    #[export] Program Instance twp_as_cif {b} s E e Φ :
+        AsCif CON (λ _, atwp b s E e Φ)%I := AS_CIF (cif_twp s E e Φ) _.
+    Next Obligation. move=>/= >. by rewrite sem_cif_in. Qed.
+  End customC.
+
+End custom_wp.
